proof/examples/zk/W64_exp_proof_5.ec
@@ -30,8 +30,8 @@ module M5 = {
 
     ctr <- W64.size - 1;
     p <- d;
-    (x1,x3) <- as_bool d ? (x3,x1) : (x1,x3);
-    (x2,x4) <- as_bool d ? (x4,x2) : (x2,x4);
+    (x1,x3) <@ ASpecFp.swapw (x1,x3,as_bool d);
+    (x2,x4) <@ ASpecFp.swapw (x2,x4,as_bool d); 
 
     while (0 < ctr) {
       ctr <- (ctr - 1);
@@ -40,14 +40,14 @@ module M5 = {
       t2 <@ ASpecFp.ith_bit(n, ctr);
       d <-  d `|` t2;
       par <- t1 `^` t2;
-      (x1,x2) <- if as_bool par then (x2,x1) else (x1, x2);
+      (x1,x2) <@ ASpecFp.swapw (x1,x2,as_bool par); 
       x1 <@ ASpecFp.mulmw64(x1,x2); 
       x2 <@ ASpecFp.mulmw64(x2,x2);  
-      (x1,x3) <- as_bool (d `^` p) ? (x3,x1) : (x1,x3);
-      (x2,x4) <- as_bool (d `^` p)  ? (x4,x2) : (x2,x4);
+      (x1,x3) <@ ASpecFp.swapw (x1,x3,as_bool (d `^` p));  
+      (x2,x4) <@ ASpecFp.swapw (x2,x4,as_bool (d `^` p));   
     }
     par <@ ASpecFp.ith_bit(n,0);
-    (x1,x2) <- if ! as_bool par  then (x2,x1) else (x1, x2);    
+    (x1,x2) <@ ASpecFp.swapw (x1,x2, ! as_bool par);
     return x1;
   }  
 
@@ -62,8 +62,8 @@ module M5 = {
 
     ctr <- W64.size - 1;
     p <- d;
-    (x1,x3) <- as_bool d ? (x3,x1) : (x1,x3);
-    (x2,x4) <- as_bool d ? (x4,x2) : (x2,x4);
+    (x1,x3) <@ M.swap_0(x1,x3,d);
+    (x2,x4) <@ M.swap_0(x2,x4,d);
 
     while (0 < ctr) {
       ctr <- (ctr - 1);
@@ -72,14 +72,14 @@ module M5 = {
       t2 <@ M.__ith_bit64(n, W64.of_int ctr);
       d <-  d `|` t2;
       par <- t1 `^` t2;
-      (x1,x2) <- if as_bool par then (x2,x1) else (x1, x2);
+      (x1,x2) <@ M.swap_0(x1,x2,par);  
       x1 <@ M.mulm(m,x1,x2); 
       x2 <@ M.mulm(m,x2,x2);  
-      (x1,x3) <- as_bool (d `^` p) ? (x3,x1) : (x1,x3);
-      (x2,x4) <- as_bool (d `^` p)  ? (x4,x2) : (x2,x4);
+      (x1,x3) <@ M.swap_0(x1,x3,(d `^` p));
+      (x2,x4) <@ M.swap_0(x2,x4,(d `^` p)); 
     }
     par <@ M.__ith_bit64(n,W64.of_int 0);
-    (x1,x2) <- if ! as_bool par  then (x2,x1) else (x1, x2);    
+    (x1,x2) <@ M.swap_0 (x1,x2, (par = W64.one) ? W64.zero : W64.one);
     return x1;
   }  
 
@@ -87,12 +87,11 @@ module M5 = {
 }.
 
 
-
-
 lemma exp_4_5' :
  equiv[ M4.expm ~ M5.expm'  : ={arg} ==> ={res}].
 proc.
 inline ASpecFp.mulmw64.
+inline ASpecFp.swapw.
 inline ASpecFp.ith_bit.
     wp.
     wp.
@@ -102,15 +101,36 @@ wp.  skip. progress.
 qed.
 
 
-(* minu_one  twos_compl to_uint_and_mod*)
 
+lemma exp_swap :
+ equiv[ M.swap_0 ~ ASpecFp.swapw    : arg{2}.`1 = arg{1}.`1 /\ arg{2}.`2 = arg{1}.`2 /\   arg{1}.`3 = as_word arg{2}.`3
+    ==> ={res}].
+proof. 
+proc.  wp. skip.
+progress.
+rewrite /set0_64. simplify.
+case (toswap{2}). progress.
+rewrite /as_word. simplify.
+smt (@W64).
+rewrite /as_word. simplify.
+smt (@W64).
+progress.
+rewrite /as_word. simplify.
+smt (@W64).  
+rewrite /as_word. simplify.
+smt (@W64).  
+qed.
+
+
+
+(* minu_one  twos_compl to_uint_and_mod*)
 lemma qqq x : 0 < x < 64 => W64.one.[x] = false.
 admit. (* progress. timeout 20. smt. *)
 qed.
 
 lemma exp_ithbit :
  equiv[ M.__ith_bit64 ~ ASpecFp.ith_bit    : arg{2}.`1 = arg{1}.`1 /\  arg{2}.`2 = W64.to_uint arg{1}.`2 
-    /\ 0 <= ctr{2} < 64 ==> ={res}].
+    /\ 0 <= ctr{2} < 64 ==> ={res} /\ (res{2} = W64.one \/ res{2} = W64.zero) ].
     symmetry.
 proc. 
 wp. skip. 
@@ -153,6 +173,7 @@ case (x = 0).
 progress. smt. 
 progress. 
 smt (qqq).
+smt().
 qed.    
 
 
@@ -161,23 +182,38 @@ lemma exp_4_5'' :
 symmetry.
 proc. 
 wp. 
+call exp_swap.
 call exp_ithbit.
-while (={ctr, n,  x1,x2,  x3, x4, d, p} /\ ImplWord m{1} P /\  0 <= ctr{1} < 64).
+while ((d{2} = W64.one \/ d{2} = W64.zero) /\ ={ctr, n,  x1,x2,  x3, x4, d, p} /\ ImplWord m{1} P /\  0 <= ctr{1} < 64).
+call exp_swap.
+call exp_swap.
  wp. 
 call mulm_specw64.
 call mulm_specw64. 
+call exp_swap.
 wp. 
 call exp_ithbit.
 call exp_ithbit.
 wp.
 skip. 
-progress. smt . smt. smt(). smt().
+progress. smt . smt. smt(). smt().  smt(@W64).
+rewrite /as_word.
+rewrite /as_bool.  smt(@W64). smt(@W64).
 wp. 
+call exp_swap.
+call exp_swap.
+wp.
 call mulm_specw64. 
 wp.
 call exp_ithbit. 
 skip.
 progress.
+rewrite /as_word.
+rewrite /as_bool.
+smt().
+rewrite /as_word.
+rewrite /as_bool.
+smt().
 qed.
 
 
